progs/verif_nest2.v
@@ -1,7 +1,13 @@
 Require Import floyd.proofauto.
 Require Import progs.nest2.
 
+Instance CompSpecs : compspecs := compspecs_program prog.
+Instance CS_legal : compspecs_legal CompSpecs.
+Proof. prove_CS_legal. Qed.
+
 Local Open Scope logic.
+
+Definition t_struct_b := Tstruct _b noattr.
 
 Definition get_spec :=
  DECLARE _get
@@ -39,14 +45,28 @@ Lemma body_get:  semax_body Vprog Gprog f_get get_spec.
 Proof.
 start_function.
 name i _i.
+destruct v as [a [b c]]; simpl in *.
+ unfold t_struct_b.
+ repeat (rewrite repinj_ind; simpl; unfold fold_reptype, unfold_reptype', eq_rect_r; rewrite <- ?eq_rect_eq).
+unfold data_at.
+unfold_field_at 1%nat. (* THIS LINE SHOULD NOT BE NECESSARY *)
+(*unfold_field_at 2%nat.*)
+normalize.
 forward.
 forward.
+ repeat (rewrite repinj_ind; simpl; unfold fold_reptype, unfold_reptype', eq_rect_r; rewrite <- ?eq_rect_eq).
+unfold data_at. unfold_field_at 3%nat. cancel. (* THIS LINE SHOULD NOT BE NECESSARY *)
 Qed.
 
 Lemma body_set:  semax_body Vprog Gprog f_set set_spec.
 Proof.
  start_function.
 name i_ _i.
+destruct v as [a [b c]]; simpl in *.
+repeat (rewrite repinj_ind; simpl; unfold fold_reptype, unfold_reptype', eq_rect_r; rewrite <- ?eq_rect_eq).
 forward.
 forward.
+unfold update22. simpl.
+repeat (rewrite repinj_ind; simpl; unfold fold_reptype, unfold_reptype', eq_rect_r; rewrite <- ?eq_rect_eq).
+cancel.
 Qed.
