floyd/proofauto.v
@@ -8,6 +8,7 @@ Require Export floyd.forward.
 Require Export floyd.call_lemmas.
 Require Export floyd.forward_lemmas.
 Require Export floyd.for_lemmas.
+Require Export floyd.nested_pred_lemmas.
 Require Export floyd.nested_field_lemmas.
 Require Export floyd.efield_lemmas.
 Require Export floyd.mapsto_memory_block.
